VST-introduction/verif_simple_kfree_file_v2.v
@@ -188,7 +188,7 @@ Definition pointer_le_bool (p q : val) : bool :=
 Fixpoint freelistrep (sh: share) (n: nat) (p: val) : mpred :=
  match n with
  | S n' => EX next: val, 
-        !! malloc_compatible (sizeof t_run) p &&  (* p is compatible with a memory block of size sizeof theader. *)
+        !! malloc_compatible (PGSIZE) p &&  (* p is compatible with a memory block of size sizeof theader. *)
         data_at sh t_run next p * (* at the location p, there is a t_run structure with the value next *)
         freelistrep sh n' next (* "*" ensures no loops... *)
  | O => !! (p = nullval) && emp
@@ -241,7 +241,7 @@ Lemma freelistrep_nonnull: forall n sh x,
    x <> nullval ->
    freelistrep sh n x =
    EX m : nat, EX next:val,
-          !! (n = S m) && !! malloc_compatible (sizeof t_run) x && data_at sh t_run next x * freelistrep sh m next.
+          !! (n = S m) && !! malloc_compatible (PGSIZE) x && data_at sh t_run next x * freelistrep sh m next.
 Proof.
    intros; apply pred_ext.
    - destruct n. 
@@ -281,7 +281,7 @@ Definition add_offset (p: val) (ofs: Z) : val :=
 Fixpoint available (sh: share) (n: nat) (p: val) (size: Z) : mpred :=
   match n with
   | S n' => 
-      !! malloc_compatible (sizeof t_run) p &&  (* Check memory compatibility *)
+      !! malloc_compatible (PGSIZE) p &&  (* Check memory compatibility *)
       data_at sh t_run nullval p *            (* Store null value *)
       available sh n' (add_offset p size) size (* Move to the next slot *)
   | O => !! (p = nullval) && emp
@@ -339,7 +339,7 @@ Lemma available_nonnull: forall n sh x size,
    x <> nullval ->
    available sh n x size =
    EX m : nat, 
-          !! (n = S m) && !! malloc_compatible (sizeof t_run) x && data_at sh t_run nullval x * available sh m (add_offset x size) size.
+          !! (n = S m) && !! malloc_compatible (PGSIZE) x && data_at sh t_run nullval x * available sh m (add_offset x size) size.
 Proof.
    intros; apply pred_ext.
    - destruct n. 
@@ -360,7 +360,7 @@ Qed.
 Lemma available_S:
   forall sh n p size,
     available sh (S n) p size =
-    !! malloc_compatible (sizeof t_run) p &&
+    !! malloc_compatible (PGSIZE) p &&
     data_at sh t_run nullval p * available sh n (add_offset p size) size.
 Proof.
   intros. simpl. reflexivity.
@@ -632,7 +632,7 @@ Admitted.*)
          PARAMS (new_head) GLOBALS(gv)
          SEP (
             freelistrep sh n original_freelist_pointer *
-            (!! malloc_compatible (sizeof t_run) new_head &&
+            (!! malloc_compatible (PGSIZE) new_head &&
             data_at sh (t_run) nullval new_head *
             data_at sh t_struct_kmem (Vint (Int.repr xx), original_freelist_pointer) (gv _kmem) )
          )
@@ -680,7 +680,7 @@ Definition freerange_no_loop_no_add_spec :=
          SEP (
             denote_tc_test_order new_head pa_end &&
             (freelistrep sh n original_freelist_pointer *
-            (!! malloc_compatible (sizeof t_run) new_head &&
+            (!! malloc_compatible (PGSIZE) new_head &&
             data_at sh (t_run) nullval new_head *
             data_at sh t_struct_kmem (Vint (Int.repr xx), original_freelist_pointer) (gv _kmem) ))
          )
@@ -693,7 +693,7 @@ Definition freerange_no_loop_no_add_spec :=
                data_at sh t_struct_kmem (Vint (Int.repr xx), new_head) (gv _kmem)
             else
                freelistrep sh n original_freelist_pointer *
-               (!! malloc_compatible (sizeof t_run) new_head &&
+               (!! malloc_compatible (PGSIZE) new_head &&
                data_at sh (t_run) nullval new_head *
                data_at sh t_struct_kmem (Vint (Int.repr xx), original_freelist_pointer) (gv _kmem) )
          ).
@@ -714,7 +714,7 @@ Definition freerange_no_loop_no_add_1_spec :=
          SEP (
             denote_tc_test_order ((Vptr b (Ptrofs.add p (Ptrofs.repr (PGSIZE))))) pa_end &&
             (freelistrep sh n original_freelist_pointer *
-            (!! malloc_compatible (sizeof t_run) (Vptr b p) &&
+            (!! malloc_compatible (PGSIZE) (Vptr b p) &&
             data_at sh (t_run) nullval (Vptr b p) *
             data_at sh t_struct_kmem (Vint (Int.repr xx), original_freelist_pointer) (gv _kmem) ))
          )
@@ -727,7 +727,7 @@ Definition freerange_no_loop_no_add_1_spec :=
                data_at sh t_struct_kmem (Vint (Int.repr xx), (Vptr b p)) (gv _kmem))
             else
                (freelistrep sh n original_freelist_pointer *
-               (!! malloc_compatible (sizeof t_run) (Vptr b p) &&
+               (!! malloc_compatible (PGSIZE) (Vptr b p) &&
                data_at sh (t_run) nullval (Vptr b p) *
                data_at sh t_struct_kmem (Vint (Int.repr xx), original_freelist_pointer) (gv _kmem)))
          ).
