VST-introduction/ASI_kalloc.v
@@ -1,10 +1,6 @@
+(** abstract spec interface *)
 Require Import VST.floyd.proofauto.
 Require Import VC.helper.
-(*Require Export malloc_lemmas.*) (*Exports the model (constants like WA , plus lemmas)*)
-
-(*Require Import malloc. needed for function and type names but not for compspecs 
-Update: Some UPenn grad students proposed to abstract over function identifiers -
-doing so in our setup makes ASIs source-program-independent!*)
 
 Global Open Scope funspec_scope.
 
@@ -21,30 +17,9 @@ Record KallocFreeAPD := {
   mem_mgr: globals -> mpred;
 }.
 
-(*Definition kalloc_token {cs:compspecs} K (sh: share) (t: type) (p: val): mpred := 
-   !! field_compatible t [] p && 
-   kalloc_token' K sh (sizeof t) p.
-
-Lemma kalloc_token_valid_pointer: forall {cs: compspecs} K sh t p, 
-      kalloc_token K sh t p |-- valid_pointer p.
-Proof. intros. unfold kalloc_token.
- apply andp_left2. apply kalloc_token'_valid_pointer.
-Qed.
-
-*)#[export] Hint Resolve kalloc_token'_valid_pointer : valid_pointer. (*
-#[export] Hint Resolve kalloc_token_valid_pointer : valid_pointer.
-
-Lemma kalloc_token_local_facts:  forall {cs: compspecs} K sh t p,
-      kalloc_token K sh t p |-- !! (field_compatible t [] p /\ malloc_compatible (sizeof t) p).
-Proof. intros.
- unfold kalloc_token.
- normalize. rewrite prop_and.
- apply andp_right. apply prop_right; auto.
- apply kalloc_token'_local_facts.
-Qed.*)
+#[export] Hint Resolve kalloc_token'_valid_pointer : valid_pointer. 
 
 #[export] Hint Resolve kalloc_token'_local_facts : saturate_local.
-(*#[export] Hint Resolve kalloc_token_local_facts : saturate_local.*)
 
 Section Kalloc_ASI.
 Variable K: KallocFreeAPD.
@@ -54,7 +29,7 @@ Variable kfree1ID: ident.
 
 Definition kfree1_spec := 
   DECLARE kfree1ID
-      WITH t:type, new_head:val, gv:globals (*sh : share, new_head:val, original_freelist_pointer:val, xx:Z, gv:globals, ls : list val, size:Z, n:Z (* n = PGSIZE.. *)*)
+      WITH t:type, new_head:val, gv:globals 
       PRE [ tptr tvoid]
         PROP(
               is_pointer_or_null new_head
@@ -75,7 +50,7 @@ Definition kfree1_spec :=
 
 Definition kalloc1_spec :=
 DECLARE kalloc1ID
-WITH t:type, gv:globals (*sh : share, original_freelist_pointer:val, xx:Z, ls:list val, gv:globals, n:Z*) (* n = PGSIZE.. *)
+WITH t:type, gv:globals 
 PRE [ ]
     PROP(0 <= sizeof t <= PGSIZE;
     complete_legal_cosu_type t = true;
@@ -85,7 +60,7 @@ PRE [ ]
 POST [ tptr tvoid ]
   EX p:val,
     PROP()
-    RETURN (p) (* we return the head like in the pop function*)
+    RETURN (p) 
     SEP (
       mem_mgr K gv;
       if eq_dec p nullval then emp
